## 2.1 A little bit about functions

> [!lemma] Lemma 2.1.2: Associativity of function composition $\circ$ (p40)
> Let $A,B,C$ and $D$ be sets and let $h : A \to B$, $g : B \to C$ and $f : C \to D$ be functions. Then
>
> $$
> \boxed{(f \circ g) \circ h = f \circ (g \circ h)}
> $$

> [!definition] Injectivity
> A function $f : A \to B$ is called **injective** if and only if
>
> $$
> \forall a_1,a_2 \in A: \boxed{f(a_1) = f(a_2) \Rightarrow a_1 = a_2} \quad \iff \quad \forall a_1,a_2 \in A: a_1 \neq a_2 \Rightarrow f(a_1) \neq f(a_2)
> $$

> [!definition] Surjectivity
> A function $f : A \to B$ is called **surjective** if and only if
>
> $$
> \forall b \in B: \boxed{\exists a \in A: f(a) = b}
> $$

> [!definition] Bijectivity
> A function $f : A \to B$ is called **bijective** if and only if it is both injective and surjective.
>
> $$
> \begin{align}
> f \text{ is bijective } &\iff f \text{ is injective and } f \text{ is surjective } \\
> &\iff \forall b \in B: \exists ! a \in A: f(a) = b \\
> \end{align}
> $$

> [!definition] Definition 2.1.3: Inverse Function (p42)
> Let $f : A \to B$ be a function. A function $g : B \to A$ is called _the_ **inverse** of $f$ if
>
> $$
> \boxed{f \circ g = id_B \quad \textbf{ and } \quad g \circ f = id_A}
> $$
>
> We denote the inverse of $f$ by $f^{-1}$.

> [!lemma] Lemma 2.1.4: A function is invertible if and only if it is bijective (p43)
> Let $f : A \to B$ be a function.
> $$\boxed{f \text{ is bijective } \iff f \text{ is invertible }}$$

> [!lemma] Lemma 2.1.5: About cardinalities of the domain and codomain of functions (p43)
> Suppose that $A$ and $B$ are sets and let $f : A \to B$ be a function.
>
> -   If $f$ is injective, then $|A| \leq |B|$.
> -   If $f$ is surjective, then $|A| \geq |B|$.

> [!lemma] Lemma 2.1.6 (p44)
> Let $A$ and $B$ be finite sets and let $f : A \to B$ be a function.
>
> $$\boxed{|A| = |B| \quad \implies \quad \big(f \text{ is injective} \iff f \text{ is surjective} \iff f \text{ is bijective}\big)}$$

## 2.2 Definition of permutations

> [!definition] Permutation (p44)
> A **permutation** of a set $A$ is a **bijective** function $f : A \to A$.

> [!definition] Definition 2.2.1: Set of permutations (p45)
> Let $A$ be a set. The set of all permutations $f: A \to A$ is denoted by $S_A$.
> In case $A = \{1,2,\ldots,n\}$ we write $S_n$ instead of $S_{\{1,2,\ldots,n\}}$.

We can write down a permutation $f \in S_n$ in two-line notation as

$$
\begin{pmatrix}
a_1 & a_2 & \cdots & a_n \\
f[a_1] & f[a_2] & \cdots & f[a_n]
\end{pmatrix}
$$

> [!definition] Composition of permutations (p46)
> If we have two permutations $f$ and $g$ on the **same** set $A$, then we can compose them to get a new **permutation** $f \circ g$ **on $A$**:
>
> $$
> (f \circ g)[a] := f[g[a]] \text{ is a permutation on } A
> $$

**Proof**
To see that $f \circ g$ is a **_function from $A$ to $A$_**, we note that since $g$ is a function from $A$ to $A$, for every $a \in A$, $g[a]$ is well-defined and belongs to $A$. Then, since $f$ is also a function from $A$ to $A$, applying $f$ to $g[a]$ gives us $(f \circ g)[a] = f[g[a]]$, which is also in $A$. Thus, for every $a \in A$, $(f \circ g)[a]$ is well-defined and belongs to $A$, confirming that $f \circ g$ is indeed a function from $A$ to $A$.

To see that $f \circ g$ is **_bijective_**, we can use Lemma 2.1.4: since both $f$ and $g$ are bijective, they both have inverses, denoted by $f^{-1}$ and $g^{-1}$. We can then check that
$$(f \circ g) \circ (g^{-1} \circ f^{-1}) = id_A \quad \text{ and } \quad (g^{-1} \circ f^{-1}) \circ (f \circ g) = id_A$$
which shows that $f \circ g$ has an inverse
$$(f \circ g)^{-1} = (g^{-1} \circ f^{-1}),$$
and from Lemma 2.1.4 it follows that $f \circ g$ is indeed bijective.

Since a bijective function from a set to itself is a permutation, we conclude that $f \circ g$ is indeed a permutation on $A$.

> [!notation] Composing a permutation with itself (p47)
> If $f$ is a permutation on a set $A$, then we denote:
>
> -   $f^0 := id_A$
> -   $f^2 := f \circ f$
> -   ...
> -   $f^k := \underbrace{f \circ f \circ \cdots \circ f}_{k \text{ times}}$

> [!definition] Order of a permutation (p47)
> Let $f$ be a permutation on a set $A$. The **order** of $f$ is defined as:
>
> $$
> \boxed{\operatorname{ord}(f) = \text{the smallest } i \in \Z_{\geq 0} \text{ such that } f^i = id_A}
> $$
>
> If no such $i$ exists, then we say that $f$ has **infinite order** and write $$\boxed{\operatorname{ord}(f) = \infty}$$

> [!theorem] Theorem 2.2.7: Central properties of composition of permutations (p47-48)
> Let $A$ be a set and $S_A$ the set of permutations on $A$. Further denote by $\circ$ the composition of permutations on $S_A$. Then we have:
>
> 1. The composition map is associative: $$\forall f,g,h \in S_A: (f \circ g) \circ h = f \circ (g \circ h)$$
> 2. The identity permutation satisfies: $$\forall f \in S_A: f \circ id_A = id_A \circ f = f$$
> 3. **There exists an inverse for every permutation** $f$, denoted by $f^{-1}$: $$\forall f \in S_A: \exists g \in S_A: g \circ f = f \circ g = id_A$$

> [!definition] Definition 2.2.8: Symmetric group on $A$ and on $n$ letters (p48)
> The pair $(S_A, \circ)$ is called the **symmetric group** on the set $A$.
> In case $A = \{1,2,\ldots,n\}$, we say that $(S_n, \circ)$ is the **symmetric group on $n$ letters**.

## 2.3 Cycle notation

> [!definition] $m$-cycle (p48)
> Let $m \geq 1$ be an integer. A permutation $f \in S_A$ is called an **$m$-cycle** if there exist $m$ distinct elements $a_0,a_1,\ldots,a_{m-1} \in A$ such that
>
> $$
> \left\{\begin{align}
> f[a_i] & = a_{(i+1) \bmod m} &\text{ for } i = 0,1,\ldots,m-1 \\
> f[x] & = x & \text{ for all } x \in A \setminus \{a_0,a_1,\ldots,a_{m-1}\}
> \end{align}\right.
> $$

That is to say,

$$
f[a_0] = a_1, \quad f[a_1] = a_2, \quad \ldots, \quad f[a_{m-2}] = a_{m-1}, \quad f[a_{m-1}] = a_0
$$

and $f$ leaves all elements in $A \setminus \{a_0,a_1,\ldots,a_{m-1}\}$ fixed.

> [!notation] Cycle notation (p49)
> If $f$ is an $m$-cycle as in the definition above, then we write $f$ in **cycle notation** as
>
> $$
> f = (a_0 \, a_1 \, a_2 \, \ldots \, a_{m-1})
> $$

> [!lemma] Lemma 2.3.2: An $m$-cycle has **order $m$** (p49)
> Let $m \geq 1$ be an integer and let $a_0, a_1, \ldots, a_{m-1}$ be distinct elements of $A$. Then the **$m$-cycle** $(a_0 \, a_1 \, a_2 \, \ldots \, a_{m-1})$ **has order $m$.**
>
> $$
> \boxed{\text{An } m\text{-cycle } (a_0 \, a_1 \, a_2 \, \ldots \, a_{m-1}) \text{ has }\textbf{order } m}
> $$

> [!definition] Mutually disjoint cycles (p49)
> Two cycles $(a_0 \, a_1 \, \ldots \, a_{m-1})$ and $(b_0 \, b_1 \, \ldots \, b_{k-1})$ are **mutually disjoint** if
>
> $$
> \{a_0,a_1,\ldots,a_{m-1}\} \cap \{b_0,b_1,\ldots,b_{k-1}\} = \emptyset
> $$

> [!exam] Distribution of exponents over disjoint cycles
> If cycles are **disjoint**, we can **distribute the exponent** over the composition:
>
> $$
> \boxed{g^i = c_1^i \circ \ldots \circ c_l^i} \qquad \text{if } c_i \cap c_j = \emptyset \text{ for all } i \neq j
> $$

**Proof**: let $g = c_1 \circ c_2 \circ \cdots \circ c_l$ be a composition of mutually disjoint cycles on a set $A$. We want to show that for every element $x \in A$, $(g^i)[x] = (c_1^i \circ c_2^i \circ \cdots \circ c_l^i)[x]$.

We consider two cases based on the position of $x$:

1. **Case 1:** $x \in c_j$ for some $j \in \{1,2,\ldots,l\}$ Since the cycles are disjoint, for every $k \neq j$, $c_k$ leaves $x$ fixed. Therefore,
    $$
         (g^i)[x] = (c_1 \circ c_2 \circ \cdots \circ c_l)^i[x] = c_j^i[x]
    $$
2. **Case 2:** $x \notin c_j$ for all $j \in \{1,2,\ldots,l\}$. If $x$ is not in any of the cycles, then all cycles leave $x$ fixed. Therefore,
   $$(g^i)[x] = (c_1 \circ c_2 \circ \cdots \circ c_l)^i[x] = x$$

> [!definition] Commuting permutations
> Two permutations $f$ and $g$ on a set $A$ are said to **commute** if
>
> $$
> f \circ g = g \circ f
> $$

> [!theorem] Disjoint cycles always commute
> Let $f$ and $g$ be two permutations on a set $A$. If $f$ and $g$ are **mutually disjoint** cycles, then they commute:
>
> $$
> \boxed{f \text{ and } g \text{ are disjoint cycles} \implies f \circ g = g \circ f}
> $$

**Proof**

Let $f = (a_0 \, a_1 \, \ldots \, a_{m-1})$ and $g = (b_0 \, b_1 \, \ldots \, b_{k-1})$ be two mutually disjoint cycles on a set $A$. We want to show that $f \circ g = g \circ f$. This means that

$$
\{a_0,a_1,\ldots,a_{m-1}\} \cap \{b_0,b_1,\ldots,b_{k-1}\} = \emptyset \quad \iff \quad A \cap B = \emptyset
$$

We will show that for every element $x \in A$, $(f \circ g)[x] = (g \circ f)[x]$.
We consider three cases based on the position of $x$:

1. **Case 1:** $x \in A \Leftrightarrow x \notin B$.
   If $x \in A$, then $g[x] = x$ (since $g$ leaves elements outside its cycle fixed). Therefore,
   $(f \circ g)[x] = f[g[x]] = f[x]$ and $(g \circ f)[x] = g[f[x]] = f[x]$. Thus, $(f \circ g)[x] = (g \circ f)[x]$.

2. **Case 2:** $x \in B \Leftrightarrow x \notin A$
   If $x \in B$, then $f[x] = x$ (since $f$ leaves elements outside its cycle fixed). Therefore, $(f \circ g)[x] = f[g[x]] = f[g[x]]$ and $(g \circ f)[x] = g[f[x]] = g[x]$. Thus, $(f \circ g)[x] = (g \circ f)[x]$.

3. **Case 3:** $x \notin A$ and $x \notin B$
   If $x$ is not in either cycle, then both $f$ and $g$ leave $x$ fixed. Therefore, $(f \circ g)[x] = f[g[x]] = f[x] = x$ and $(g \circ f)[x] = g[f[x]] = g[x] = x$. Thus, $(f \circ g)[x] = (g \circ f)[x]$.

> [!theorem] Theorem 2.3.5: Disjoint cycle decomposition (p51)
> Let $n \in \N$ and let $A$ be a **finite (!)** set with cardinality $\lvert A \rvert = n$. Then every permutation $f \in S_A$ can be written as a composition of **mutually disjoint** cycles:
>
> $$f = c_1 \circ c_2 \circ \cdots \circ c_l$$

Note that the **identity permutation** $\id \in S_A$ is a composition of $n$ mutually disjoint $1$-cycles:
$$\id = (1)(2)(3)\cdots(n)$$

> [!corollary] Corollary 2.3.6: **Uniqueness** of DCD up to ordering (p52)
> Let $n \in \N$ and let $A$ be a set with cardinality $\lvert A \rvert = n$. Further let $f \neq \id \in S_A$ be a permutation _distinct from the identity_ permutation. Suppose
> $$f \quad = \quad c_1 \circ c_2 \circ \cdots \circ c_l \quad = \quad d_1 \circ d_2 \circ \cdots \circ d_k$$
> are two decompositions of $f$ into mutually disjoint cycles. Then
>
> -   $l = k$
> -   After reordering if necessary, $c_i = d_i$ for all $i = 1,2,\ldots,l$.
>     $$\boxed{\text{The disjoint cycle decomposition of } f \text{ is \textbf{UNIQUE} up to ordering of the cycles}}$$

If the <b style="color:red;">1-cycles are removed</b>, there is _essentially_ only <b style="color:red;">one way</b> to write $f$ as a composition of
mutually disjoint cycles.

The "essentially" in this statement just means that the only freedom one has is to <b style="color:red;">change ordering</b> of the cycles in the composition, which does not really matter since **disjoint cycles commute**.

> [!definition] Definition 2.3.9: Type of a permutation (p53)
> Let $A$ be a set with cardinality $\lvert A \rvert = n$ and let $f \in S_A$ be a permutation. Suppose that the disjoint cycle decomposition of $f$ has the form $f = c_1 \circ c_2 \circ \cdots \circ c_l$, where
>
> -   $f$ has $t_1$ fixed points (1-cycles),
> -   $f$ has $t_i$ $i$-cycles for $i = 2,3,\ldots,n$
>
> Then the **cycle type** of $f$ is defined as the $n$-tuple
>
> $$
> \boxed{(t_1, t_2, \ldots, t_n)} \qquad \text{for } \, \boxed{|A| = n}
> $$

If $f \in S_A$ has cycle type $(t_1, t_2, \ldots, t_n)$, then - since there are only $n$ elements in $A$ - it must hold that

$$
\boxed{t_1 + 2t_2 + 3t_3 + \cdots + n t_n = n}
$$

> [!proposition] Proposition 2.3.12: Order of a permutation based on DCD (p54)
> Let $A$ be a **finite** set with cardinality $\lvert A \rvert = n$ and let $f \in S_A$ have a disjoint cycle decomposition $f = c_1 \circ c_2 \circ \cdots \circ c_l$, where $c_i$ is an $m_i$-cycle for $i = 1,2,\ldots,l$. Then
>
> $$
> \boxed{\operatorname{ord}(f) = \operatorname{lcm}(m_1, m_2, \ldots, m_l)} \text{ where the } m_i \text{ are the lengths of the disjoint cycles in the DCD}
> $$
>
> _Example_: $\operatorname{ord}((1 \, 2 \, 3)(4 \, 5)) = \operatorname{lcm}(3,2) = 6$.

So to determine the order of a permutation, it is sufficient to know its cycle type.

## Exercises

> [!exercise] HW1.1
> $$\forall n\in\N : \forall g \in S_n : \boxed{g \text{ and } g^{-1} \text{ have the same cycle \textbf{type} and \textbf{order}}}$$

> [!exercise] HW1.2 a) and b)
> If $h \in S_n$ is an $m$-cycle, then
> $$\forall g\in S_n : \boxed{g \circ h \circ g^{-1} \text{ is also an } m\text{-cycle}}$$
> and
> $$h \text{ and } g \circ h \circ g^{-1} \text{ have the same cycle type and order}.$$

The order depends only on the cycle type (Proposition 2.3.12).

> [!exercise] HW1.2 c)
> The relation
> $$\sim \, = \{(h,k) \in S_n \times S_n \mid \exists g \in S_n : k = g \circ h \circ g^{-1}\}$$
> is an equivalence relation on $S_n$.
