## 6.1 Group homomorphisms

> [!definition] Definition 6.1.1: Group homomorphism and isomorphism
> Let $(G_1, \cdot_1)$ and $(G_2, \cdot_2)$ be groups. A function $\boxed{\psi: G_1 \to G_2}$ is a **group <u>homomorphism</u>** if it satisfies
>
> 1. $\boxed{\psi(e_1) = e_2}$
> 2. $\forall f,g \in G: \boxed{\psi(f \cdot_1 g) = \psi(f) \cdot_2 \psi(g)}$
>
> If $\psi : G_1 \to G_2$ is **bijective** as well, it is called a **group <u>isomorphism</u>**.

> [!definition] Isomorphic Groups
> Two groups $(G_1, \cdot_1)$ and $(G_2, \cdot_2)$ are called **isomorphic**
> if there exists a group isomorphism (bijective homomorphism) $\psi : G_1 \to G_2$:$$\boxed{(G_1, \cdot_1) \simeq (G_2, \cdot_2)}$$

> [!exercise] Exercise 6.13: Composition of group homomorphisms
> Let $(G_1, \cdot_1)$, $(G_2, \cdot_2)$ and $(G_3, \cdot_3)$ be groups and let $\psi_1 : G_1 \to G_2$ and $\psi_2 : G_2 \to G_3$ be group homomorphisms.
>
> -   The composition $\psi_2 \circ \psi_1 : G_1 \to G_3$ is also a group homomorphism.
> -   If both $\psi_1$ and $\psi_2$ are group **iso**morphisms, then $\psi_2 \circ \psi_1$ is also a group **iso**morphism

> [!exercise] Exercise 6.18: Isomorphism as an equivalence relation
> Being isomorphic is an equivalence relation on the set of all groups.
>
> -   Reflexive:
>     -   _$\text{id}_G : G \to G$ is a group isomorphism (**automorphism**)._
> -   Symmetric
>     -   _If $\psi : G_1 \to G_2$ is a group isomorphism, then its inverse $\psi^{-1} : G_2 \to G_1$ is also a group isomorphism._
> -   Transitive:
>     -   _**The composition of two group homomorphisms is again a group homomorphism**._
>     -   $\psi_2 \circ \psi_1 : G_1 \to G_3$ is a group homomorphism if $\psi_1 : G_1 \to G_2$ and $\psi_2 : G_2 \to G_3$ are group homomorphisms.

![[images/6/multiplication-table.jpg]]
$$h = f \cdot_1 g \qquad \text{and} \qquad \psi(h) = \psi(f) \cdot_2 \psi(g)$$

Note how similar the definition of a group **homomorphism** is to the definition of a group **action** (Def. 5.1.1).

> [!example] Example 6.1.5: A group action is a group homomorphism
> Let $(G, \cdot)$ be a group with identity element $e_1$ that acts on the set $A$ via $\varphi : G \to S_A$.
>
> -   Since $\varphi_{e_1} = \text{id}_A$ and $\text{id}_A = e_2$ is the identity element of $S_A$, we have $\varphi(e_1) = e_2$.
> -   For any $f,g \in G$ we have $\varphi_{g \cdot f} = \varphi_g \circ \varphi_f$ by definition of a group action.
>     Since $\circ = \cdot_2$ is the group operation in $S_A$, we have $\varphi(g \cdot f) = \varphi(g) \cdot_2 \varphi(f)$.
>
> We conclude: **any group action $\varphi : G \to S_A$ is a group homomorphism on $S_A$**

Lemma 5.1.2 (group actions preserve inverses) can be generalized to any group **homomorphism**:

> [!lemma] Lemma 6.1.6: Group homomorphisms preserve inverses
> Let $\psi : G_1 \to G_2$ be a group homomorphism. Then for any $f \in G_1$ we have
> $$\boxed{\psi(f^{-1}) = (\psi(f))^{-1}}$$

> [!definition] Definition 6.1.7: Kernel of a group homomorphism
> Let $\psi : G_1 \to G_2$ be a group homomorphism and let $e_2$ be the identity element of $G_2$.
> Then we define the **kernel** of $\psi$ as
> $$\boxed{\ker(\psi) := \{ g \in G_1 \mid \psi(g) = e_2 \}}$$

> [!fact] Kernel of $\psi : G_1 \to G_2$ always contains the identity element of $G_1$
> Since $\psi$ is a group homomorphism, we have $\psi(e_1) = e_2$. Therefore $$e_1 \in \ker(\psi)$$

If the kernel only contains the identity element, the homomorphism $\psi$ is injective:

> [!lemma] Lemma 6.1.8: Injectivity and kernel
> Let $\psi : G_1 \to G_2$ be a group homomorphism. Then $$\boxed{\psi \text{ is injective} \iff \ker(\psi) = \{ e_1 \}}$$

We proved this in Exercise 6.14.

> [!fact] Group <u>iso</u>morphisms have trivial kernel
> If $\psi : G_1 \to G_2$ is a group **iso**morphism, then $\psi$ is bijective and therefore injective.
> By Lemma 6.1.8, we have $$\ker(\psi) = \{ e_1 \}$$

> [!theorem] Theorem 6.1.9: Kernel is a NORMAL subgroup
> Let $\psi : G_1 \to G_2$ be a group homomorphism. Then $$\ker(\psi) \subseteq G_1 \text{ is a subgroup of } G_1$$
> Moreover,
> $$\forall f \in G_1 : \qquad \boxed{f \cdot_1 \ker(\psi) = \ker(\psi) \cdot_1 f}$$
> In other words, the kernel is a **normal subgroup** of $G_1$ (Def. 6.1.10).

> [!definition] Definition 6.1.10: Normal subgroup
> A subgroup $H$ of a group $(G, \cdot)$ is called a **<u>normal</u> subgroup** if
> $$\forall f \in G : \qquad \boxed{f \cdot H = H \cdot f}$$
> In other words, all left cosets of $H$ are equal to the corresponding right cosets.
> In normal subgroups $H$, we have that $\forall h \in H, \forall g \in G$:
> $$\boxed{g \cdot h \cdot g^{-1} \in H}$$

This last property is often used as an alternative definition of normal subgroups. Why does it hold?
**Proof**
Let $h \in H$ and $g \in G$ be arbitrary. Since $H$ is a normal subgroup, we have
$$g \cdot H = H \cdot g.$$
This implies that there exists an element $h' \in H$ such that
$$g \cdot h = h' \cdot g.$$
Multiplying both sides from the right by $g^{-1}$, we obtain
$$g \cdot h \cdot g^{-1} = h' \cdot g \cdot g^{-1} = h' \cdot e = h' \in H.$$

> [!deduction] The kernel is a normal subgroup
> It follows directly from Theorem 6.1.9 and Definition 6.1.10 that the **kernel** of any group homomorphism $\psi : G_1 \to G_2$ is a **normal** subgroup of $G_1$.

Because the **kernel is a normal subgroup**, we can prove that a subgroup $H$ of a group $G$ is normal by identifying it as the kernel of a suitable group homomorphism $\psi : G \to G_2$.

> [!definition] Definition: Image of a group homomorphism
> Let $\psi : G_1 \to G_2$ be a group homomorphism. Then we define the **image** of $\psi$ as
>
> $$
> \boxed{\text{im}(\psi) := \{ \psi(g) \mid g \in G_1 \} \subseteq G_2}
> $$

Note that the image is **never** **empty**, since $e_2$ is always in it:
$$e_1 \in G_1 \implies \psi(e_1) \eqDef \boxed{e_2 \in \text{im}(\psi)}.$$

> [!exercise] Exercise 6.15: The image is a subgroup of $G_2$
> Let $\psi : G_1 \to G_2$ be a group homomorphism. Then $$\text{im}(\psi) \subseteq G_2 \text{ is a subgroup of } G_2.$$

> [!exam] Isomorphic groups and element order
> Let $(G_1, \cdot_{1}) \simeq (G_2, \cdot_{2})$ be isomorphic via the group isomorphism $\varphi : G_1 \to G_2$.
> Then for any $g \in G_1$
>
> $$
> \boxed{\text{ord}(g) = \text{ord}(\varphi(g))}
> $$
>
> So a group isomorphism maps elements to elements of the same order.
> We can thus **check if an isomorphism can exist between two groups by comparing the orders of their elements.**

**Proof**.

Let $\ord(g) = n$ for $g \in G_1$.
$$\varphi(g)^n = \underbrace{\varphi(g) \cdot_{2} \ldots \cdot_{2} \varphi(g)}_n \stackrel{(2)}{=} \varphi(g \cdot_{1} \ldots \cdot_{1} g) = \varphi(g^{n}) \stackrel{\text{ord}(g)=n}{=} \varphi(e_{1}) \stackrel{(1)}{=} e_{2}.$$
We conclude that $\varphi(g)^n = e_{2}$, so because of Lemma 3.1.12, $\ord(\varphi(g))$ divides $n$.
Now we show that $n$ is the smallest such positive integer.

Assume there exists a positive integer $m < n$ such that $\varphi(g)^m = e_{2}$.
Then, by similar reasoning as above, we have $\varphi(g^{m}) = e_{2}$.

Now we see that $$\varphi \text{ is injective } \stackrel{\text{Lemma 6.1.8}}{\implies} \ker(\varphi) = \{ e_{1} \} \implies g^{m} = e_{1}$$But we assumed that $\ord(g) = n$ and that $m<n$. This gives a contradiction, since the order is by definition the smallest positive integer such that $g^{\ord(g)} = e_{1}$.
Therefore, no such $m$ can exist and we conclude that $\ord(\varphi(g)) = n$.

---

## 6.2 Quotient groups

We will show that a **normal** subgroup (with left cosets = right cosets) $H \subseteq G$ of a group $(G, \cdot)$ can be used to construct a new group, called the **quotient group** $G/H$.

> [!definition] Definition 6.2.1:
> Let $(G, \cdot)$ be a group and $H \subseteq G$ be a **<u>normal</u>** subgroup of $G$ we define
> $$\boxed{G/H := \{ f \cdot H \mid f \in G \}} = \{ H \cdot f \mid f \in G \}$$
> as the **set of all cosets** of $H$ in $G$.
> Its size $|G/H|$ is called the **index** of $H$ in $G$ and denoted by $[G : H]$.

Using multiplication of subsets (Def. 4.2.1), we can define a **group operation** $\cdot$ on $G/H$:$$(fH) \cdot (gH) := \{k \cdot \ell \mid k \in fH, \ell \in gH\}$$where $fH, gH \in G/H$.

> [!definition] Definition 6.2.2
> Let $(G, \cdot)$ be a group and $H \subseteq G$ be a <u>normal</u> subgroup of $(G, \cdot)$.
> Let $C,D \in G/H$ be two cosets of $H$ in $G$.
> Suppose that $f \in C$ and $g \in D$ are arbitrary representatives of $C$ and $D$, respectively.
>
> We define the **product** of the cosets $C$ and $D$ as
> $$C \cdot D := (f \cdot g)H$$
> Note that this coset is independent of the choice of representatives $f$ and $g$.

Let $f, f'$ be two representatives of the coset $C$ (i.e., $fH = f'H$).
Let $g, g'$ be two representatives of the coset $D$ (i.e., $gH = g'H$).
We must show that:
$$(f' \cdot g')H = (f \cdot g)H$$

**Step 1: Express representatives using $H$**
Since $f'$ and $f$ are in the same coset, $f'$ must equal $f$ multiplied by some element of $H$:
$$f' = f \cdot h_1 \quad \text{for some } h_1 \in H$$
Similarly for $g'$ and $g$:
$$g' = g \cdot h_2 \quad \text{for some } h_2 \in H$$

**Step 2: Examine the product $f' \cdot g'$**
Substitute the expressions from Step 1:
$$f' \cdot g' = (f \cdot h_1) \cdot (g \cdot h_2)$$

<b style="color:red;">We CANNOT simply swap </b>$\red{h_1 \cdot g \to g \cdot h_1}$
Even though $H$ is **normal**, $G$ is not necessarily abelian!

**Step 3: Utilize Normality of $H$**
We need to group $f$ and $g$ together. To do this, we must commute $h_1$ and $g$.
Since $H$ is a <u>normal</u> subgroup, we know that $Hg = gH$.
**Thus, for any $h_1 \in H$, there exists an $h_3 \in H$ such that**:
$$h_1 \cdot g = g \cdot h_3$$

**Step 4: Substitution and Conclusion**
Substitute $g \cdot h_3$ back into the main equation:
$$\begin{aligned} f' \cdot g' &= f \cdot (g \cdot h_3) \cdot h_2 \\ &= (f \cdot g) \cdot (h_3 \cdot h_2) \end{aligned}$$
Since $H$ is a subgroup, $h_3 \cdot h_2 \in H$. Let $h_{new} = h_3 \cdot h_2$.
$$f' \cdot g' = (f \cdot g) \cdot h_{new}$$
Because $f' \cdot g'$ differs from $f \cdot g$ only by an element in $H$, they generate the same coset:
$$(f' \cdot g')H = (f \cdot g)H$$

> [!exam] Utilizing normality
> Given an element $h_1 \cdot g \in H \cdot g$, we **cannot** simply swap $h_1$ and $g$ to get an element in the coset $g \cdot H$. However, since $H$ is a **normal** subgroup, we know that $Hg = gH$.
> Thus, for any $h_1 \in H$, there exists an $h_3 \in H$ such that
> $$h_1 \cdot g = g \cdot h_3.$$

> [!notation] Notation: representatives of cosets
> If $C \in G/H$ is a coset of the normal subgroup $H$ in $G$, then any $f \in C$ is called a **representative** of the coset $C$.

**Restated Definition 6.2.2**:
If $f$ is a representative of a coset $C \in G/H$ and $g$ is a representative of a coset $D \in G/H$, then $C \cdot D$ is again a coset of $H$ in $G$ (and thus $C \cdot D \in G/H$) and $f \cdot g$ is a representative of $C \cdot D$.

> [!definition] Definition 6.2.3: Quotient group
> Let $(G, \cdot)$ be a group, $H \subseteq G$ a **normal** subgroup of $G$ and $G/H$ the set of all cosets of $H$ in $G$ (Def. 6.2.1). Then the multiplication of cosets$$\boxed{(fH) \cdot (gH) := (f \cdot g)H} \quad \textit{(Def. 6.2.2)}$$ gives rise to a **group structure** on $(G/H, \cdot)$.

We can explicitly write out the group operations to clarify how they work. Let $\cdot_G$ be the group operation in $(G, \cdot_G)$ (with **normal** subgroup $H$) and $\cdot_{G/H}$ be the group operation in the quotient group $(G/H, \cdot_{G/H})$. Then
$$(fH) \cdot_{G/H} (gH) = (f \cdot_G g)H.$$

We can see that

1. The composition of left (right) cosets is again a left (right) coset.
2. The representative of the composition is the composition of the representatives.

> [!exam] Identity element of the quotient group
> Let $(G, \cdot)$ be a group, $H \subseteq G$ a **normal** subgroup of $G$ and $(G/H, \cdot)$ the quotient group.
>
> $$
> \boxed{e_{G/H} = e_G \cdot H = H}
> $$

**Proof**

By definition of the identity element in a group, we have to show that
$$(fH) \cdot H = fH = H \cdot (fH)$$
Using the definition of the group operation in the quotient group, we have
$$(fH) \cdot H = (fH) \cdot (e_G H) \eqDef (f \cdot e_G)H = fH$$
and
$$H \cdot (fH) = (e_G H) \cdot (fH) \eqDef (e_G \cdot f)H = fH.$$

> [!exam] Inverse of a left coset in the quotient group
> Let $(G, \cdot)$ be a group, $H \subseteq G$ a **normal** subgroup of $G$ and $(G/H, \cdot)$ the quotient group.
> $$ \forall f \in G : \qquad \boxed{(fH)^{-1} = (f^{-1})H} $$

**Proof**

By definition of the inverse element in a group, we have to show that
$$(fH) \cdot (f^{-1}H) = e_{G/H} = H = (H f^{-1}) \cdot (fH)$$
Using the definition of the group operation in the quotient group, we have
$$(fH) \cdot (f^{-1}H) = (f \cdot f^{-1})H = e_G H = H.$$
and the proof is completely analogous for the right side.

> [!exercise] Exercise 6.16
> Let $(G, \cdot)$ be a group. Then for the quotient group by the trivial normal subgroup $\{e_G\}$ we have
> $$\boxed{\left(G/\{e_G\}, \cdot\right) \simeq (G, \cdot)}$$
> by the isomorphism
> $$\psi : G/\{e_G\} \to G, \quad \psi(f \cdot \{e_G\}) := f$$

> [!exercise] Exercise 6.16
> If $\psi : G_1 \to G_2$ is an **injective** homomorphism, then
> $$\boxed{\left(G_1, \cdot_{G_1}\right) \simeq \left(\text{im}(\psi), \cdot_{G_2}\right)}$$
> by the isomorphism theorem and the isomorphism
> $$\overline{\psi} : G_1/\{e_1\} \to \text{im}(\psi), \quad \overline{\psi}(g \cdot \{e_1\}) = \psi(g \cdot \{e_1\}) = g$$

Where $\ker(\psi) = \{e_1\}$ because $\psi$ is injective (Lemma 6.1.8).
It follows from the isomorphism theorem (Theorem 6.3.1) that
$$(G_1 / \ker(\psi), \cdot_{G_1}) \simeq (\text{im}(\psi), \cdot_{G_2})$$
and from Exercise 6.16 that
$$(G_1 / \{e_1\}, \cdot_{G_1}) \simeq (G_1, \cdot_{G_1}).$$
Combining both results gives the desired isomorphism (since composition of isomorphisms is again an isomorphism, Exercise 6.18).

---

> [!exercise] Group Automorphisms
> A group isomorphism $\psi : G \to G$ from a group $(G, \cdot)$ to itself is called a **group automorphism**.
> The set of all group automorphisms of $(G, \cdot)$ is denoted by $\text{Aut}(G)$.
> $$(\text{Aut}(G), \circ) \text{ is a group}$$
> where $\circ$ is the composition of functions.

**Proof**

-   We already showed in Exercise 6.18 that the **composition of two group homomorphisms is again a group homomorphism.**
-   The identity function $\text{id}_G : G \to G$ is a group automorphism (Exercise 6.18).
-   The inverse of a group automorphism is again a group automorphism (Exercise 6.18).
-   Composition of functions is associative (function composition is associative by Lemma 2.1.2)

---

## 6.3 The isomorphism theorem

> [!theorem] Theorem 6.3.1: The isomorphism theorem
> Let $\psi : G_1 \to G_2$ be a group <u>homo</u>morphism. Then the map
> $$\boxed{\overline{\psi} : \begin{cases}G_1/\ker(\psi) \to \text{im}(\psi)\\ \, \, \, \, g \cdot \ker(\psi) \mapsto \psi(g)\end{cases}}$$
> is a group **<u>iso</u>morphism**. In other words,
>
> $$
> \boxed{\left(G_1 / \ker(\psi), \cdot_{G_1 / \ker(\psi)}\right) \simeq \left(\text{im}(\psi), \cdot_{G_2}\right)}
> $$

Here, $G_1 / \ker(\psi)$ is the quotient group of $G_1$ by the kernel of $\psi$:

-   $\ker(\psi) \subseteq G_1$ is a **normal** subgroup of $G_1$ by Theorem 6.1.9.
-   $G_1 / \ker(\psi)$ is thus a **quotient** group (Def. 6.2.3).
-   $|G_1 / \ker(\psi)| = [G_1 : \ker(\psi)]$ is the index of $\ker(\psi)$ in $G_1$ (Def. 6.2.1).
-   By Langrange's theorem (Theorem 4.3.3), if **$G$ is finite**, then$$|G_1 / \ker(\psi)|=[G_1 : \ker(\psi)] = \frac{|G_1|}{|\ker(\psi)|}.$$

> [!fact] 'Well-defined' map
> To show that a map $f : A \to B$ is **well-defined**, one has to show that $\forall a,b \in A$:
> $$a = b \implies f(a) = f(b)$$

![[images/6/group-isomorphism.jpg]]
